Finished? Host

Host.v.dfy
@@ -37,7 +37,45 @@ module Host {
 /*{*/
   // Replace these definitions with more meaningful ones that capture the operations
   // of a key-value store described above.
-  datatype Constants = Constants()
-  datatype Variables = Variables()
+  datatype Constants = Constants() 
+  datatype Variables = Variables(hostOwnedMap: imap <int, int>)
+
+
+  ghost predicate GroupInit(grp_c: seq<Constants>, grp_v: seq<Variables>) {
+    && |grp_v| > 0 // Not sure if we need this, but keeping in for my paranioa 
+    && forall idx | 0 <= idx < |grp_v| :: grp_v[idx].hostOwnedMap == if idx == 0 then ZeroMap() else EmptyMap() //is zero map correct here?
+  }
+
+  ghost predicate SendMessage(c: Constants, v: Variables, v': Variables, event: Event, msgOps:Network.MessageOps) {
+    && msgOps.send.Some? 
+    && msgOps.recv.None? 
+    && var keySet := msgOps.send.value.sentMap.Keys; //set of keys needed for the remove
+    && (forall k :: (k) in msgOps.send.value.sentMap ==> (k in v.hostOwnedMap) && msgOps.send.value.sentMap[k] == v.hostOwnedMap[k]) //need some way to check that we have what we are sending!!!
+    && v'.hostOwnedMap == MapRemove(v.hostOwnedMap, keySet) //and then remove it from 
+  } 
+
+
+  ghost predicate ReceiveMessage(c: Constants, v: Variables, v': Variables, event: Event, msgOps: Network.MessageOps) {
+    && msgOps.send.None? 
+    && msgOps.recv.Some? 
+    && v'.hostOwnedMap == IMapUnionPreferLeft(msgOps.recv.value.sentMap, v.hostOwnedMap) //just take it in
+  }
+
+  ghost predicate Next(c: Constants, v: Variables, v': Variables, event: Event, msgOps: Network.MessageOps)
+    {
+      match event {
+      case Get(key, value) =>
+        && key in v.hostOwnedMap
+        && value == v.hostOwnedMap[key]
+        && v' == v
+    
+      case Put(key, value) =>
+        && v'.hostOwnedMap == v.hostOwnedMap[key := value]
+        
+      case NoOp => SendMessage(c, v, v', event, msgOps) || ReceiveMessage(c, v, v', event, msgOps)
+
+      }
+    }
+
 /*}*/
 }
